Congruence_Closure_Explain/CC_Termination.thy
@@ -1,0 +1,151 @@
+section \<open>Termination proof for congruence closure\<close>
+theory CC_Termination
+  imports CC_Invars
+begin 
+
+abbreviation root_set where
+  "root_set l \<equiv> {i | i. i < length l \<and> l ! i = i}"
+
+
+definition nr_eq_classes :: "nat list \<Rightarrow> nat"
+  where "nr_eq_classes l = card (root_set l)"
+
+lemma ufa_union_decreases_nr_eq_classes:
+  assumes "ufa_invar l" "a < length l" 
+    "rep_of l a \<noteq> rep_of l b"
+shows "nr_eq_classes (ufa_union l a b) = nr_eq_classes l - 1"
+proof-
+  have "rep_of l a \<in> root_set l"
+    by (simp add: assms rep_of_less_length_l rep_of_root)
+  have "root_set l = root_set (ufa_union l a b) \<union> {rep_of l a}"
+    by (auto simp add: nth_list_update' assms rep_of_bound rep_of_min \<open>rep_of l a \<in> root_set l\<close>)
+  moreover have "rep_of l a \<notin> root_set (ufa_union l a b)"
+    using assms by auto
+  ultimately show ?thesis unfolding nr_eq_classes_def
+    by simp
+qed
+
+lemma nr_eq_classes_gt_0:
+  assumes "ufa_invar l" "length l > 0"
+  shows "nr_eq_classes l > 0"
+proof(rule ccontr)
+  assume "\<not> 0 < nr_eq_classes l"
+  then have no_eq_classes: "nr_eq_classes l = 0"
+    by blast
+  then obtain i where i: "i < length l" 
+    using assms by auto
+  have "\<not> rep_of_dom (l, i)"
+    using assms(1) i assms(2) proof(induction rule: rep_of_induct)
+    case (base i)
+    then have "l ! i \<noteq> i" 
+      using no_eq_classes unfolding nr_eq_classes_def by simp
+    then show ?case 
+      using base by blast
+  next
+    case (step i)
+    then show ?case 
+      using rep_of_domain by auto
+  qed
+  then show "False" 
+    using assms(1) i ufa_invarD(1) by auto
+qed
+
+lemma propagate_domain:
+  assumes "cc_invar cc" "nr_vars cc > 0"
+  shows "propagate_dom cc"
+  using assms proof(induction "nr_eq_classes (cc_list cc)" arbitrary: cc)
+  case 0
+  then have "0 < nr_eq_classes (cc_list cc)" 
+    using nr_eq_classes_gt_0 unfolding cc_list_invar_def by blast
+  then show ?case
+    using 0 by linarith
+next
+  case (Suc x)
+  then show ?case 
+  proof(cases "pending cc")
+    case Nil
+    then show ?thesis using propagate.domintros 
+      by (metis congruence_closure.cases congruence_closure.select_convs(4))
+  next
+    case (Cons eq pe)
+    define a b where a_b: "a = left eq" "b = right eq"
+    obtain l u t pf pfl ip where 
+      cc: "cc = \<lparr>cc_list = l, use_list = u, lookup = t, pending = (eq # pe), proof_forest = pf, pf_labels = pfl, input = ip\<rparr>"
+      using Cons  by (metis congruence_closure.cases congruence_closure.select_convs(4))
+    then show ?thesis proof(cases "rep_of l a = rep_of l b")
+      case True
+      let ?step = "\<lparr>cc_list = l, use_list = u, lookup = t, pending = pe, proof_forest = pf, pf_labels = pfl, input = ip\<rparr>"
+      have "cc_invar ?step" 
+        using Suc.prems(1) True a_b(1) a_b(2)cc cc_invar_step2 by blast
+      then have "propagate_dom ?step" using True Suc(1)
+      proof (induction pe)
+        case Nil
+        then show ?case using propagate.domintros by blast
+      next
+        case (Cons eq2 pe2)
+        then show ?case proof(cases "rep_of l (left eq2) = rep_of l (right eq2)")
+          case True
+          let ?step = "\<lparr>cc_list = l, use_list = u, lookup = t, pending = pe2, proof_forest = pf, pf_labels = pfl,
+        input = ip\<rparr>" 
+          from True have *: "cc_invar ?step" using cc_invar_step2
+            using Cons.prems(1) by blast
+          with Cons have "propagate_dom ?step"
+            by blast
+          then show ?thesis using propagate.domintros Cons True by presburger
+        next
+          case False
+          let ?step = "(propagate_step l u t pe2 pf pfl ip (left eq2) (right eq2) eq2)"
+          have *: "cc_list ?step = ufa_union l (left eq2) (right eq2)" by (simp add: cc_list_loop)
+          have "(left eq2) < length l" "ufa_invar l"  using Cons 
+             apply (metis  pending_left_right_valid)
+            using Suc unfolding cc_list_invar_def cc by simp
+          then have "nr_eq_classes (ufa_union l (left eq2) (right eq2)) = nr_eq_classes l - 1" 
+            using ufa_union_decreases_nr_eq_classes Suc * False by blast 
+          then have "propagate_dom ?step"
+            by (metis "*" Cons.prems(1) False Suc.hyps(1) Suc.hyps(2) Suc.prems(2) cc cc_invar_step congruence_closure.select_convs(1) diff_Suc_1 length_list_update)
+          then show ?thesis using propagate.domintros 
+            using False by presburger
+        qed
+      qed
+      then show ?thesis using cc propagate.domintros True a_b by blast
+    next
+      case False
+      let ?step = "(propagate_step l u t pe pf pfl ip a b eq)"
+      have *: "cc_list ?step = ufa_union l a b" 
+        by (simp add: cc_list_loop)
+      have "a < length l" "ufa_invar l" using a_b Suc 
+         apply (metis cc pending_left_right_valid)
+        using Suc unfolding cc_list_invar_def cc by simp
+      then have "nr_eq_classes (ufa_union l a b) = nr_eq_classes l - 1" 
+        using ufa_union_decreases_nr_eq_classes Suc * False by blast 
+      then have "propagate_dom ?step"
+        using Suc False a_b cc cc_invar_step cc_list_loop by auto
+      then show ?thesis using cc propagate.domintros False a_b by blast
+    qed
+  qed
+qed
+
+lemma valid_vars_imp_nr_vars_gt_0:
+  assumes "valid_vars eq (nr_vars cc)"
+  shows "nr_vars cc > 0"
+proof(cases eq)
+  case (Constants x11 x12)
+  with assms have "x11 < nr_vars cc" 
+    by simp
+  then show ?thesis 
+    by simp
+next
+  case (Function x21 x22 x23)
+  with assms have "x21 < nr_vars cc" 
+    by simp
+  then show ?thesis 
+    by simp
+qed
+
+corollary propagate_domain':
+  assumes "cc_invar cc" "valid_vars eq (nr_vars cc)"
+  shows "propagate_dom cc"
+  using propagate_domain valid_vars_imp_nr_vars_gt_0 assms by blast
+
+
+end
